---
title: 贝塞尔曲线
layout: post
published: false

---

公式
--------
参数方程 t 在 0 - t 之间变化

### 1阶
B(t) = (1 - t) * P0 + (t) * P1

(1 - t) + t

### 2阶
B(t) = (1 - t)^2 * P0 + 2t(1 - t)P1 + t ^ 2 * P2

[(1 - t) + t] ^ 2 = (1 - t) ^ 2 + 2 * t (1 - t)

### 3阶
B(t) = (1 - t)^3 * P0 + 3t(1 - t)^2 P1 + 3 t ^ 2 ( 1 - t) * P2 + t ^ 3 * P3

[(1 - t) + t] ^ 3 = (1 - t)^3 + 3(1 - t)^2 * t + 2 (1 - t) * t ^ 2 + t ^ 3

4 阶，5 阶，6 阶依次类推。

杨辉三角

			  1
			 1 1
		   1  2  1
	     1  3  3  1
	        
a^2 + b^2 = c^2

<script type="math/tex; mode=display">
e^x = \sum\_{n=0}^\infty \frac{x^n}{n!} = \lim\_{n\rightarrow\infty} (1+x/n)^n 
</script>
